\section{Properties of Power Spectral Density (PSD)}One of the definitions of PSD is expressed in instruction and the power expression can be separated into conjugate product,  which is\begin{align}P(\omega) & = \lim\limits_{N \to \infty} \mathbb{E} \left\{ \frac{1}{N} \left| \sum_{n=0}^{N-1} x(n) e^{-j n \omega} \right|^2 \right\}\label{proof:periodogram:starter}\\& = \lim\limits_{N \to \infty} \mathbb{E} \left\{ \frac{1}{N} \sum_{n=0}^{N-1} x(n) e^{-j n \omega} \sum_{m=0}^{N-1} x(m)^\ast e^{j m \omega}  \right\} \notag\\& =\lim\limits_{N \to \infty} \frac{1}{N} \sum_{n=0}^{N-1} \sum_{m=0}^{N-1} \mathbb{E} \bigg \{  x(n)e^{-j n \omega}  x^*(n)e^{j m \omega}\bigg\}\notag\\& =\lim\limits_{N \to \infty} \frac{1}{N} \sum_{n=0}^{N-1} \sum_{m=0}^{N-1}	\mathbb{E} \bigg \{  x(n) x^*(n)\bigg\}e^{-j(n-m)\omega}\label{proof:periodogram}\end{align}In addition, the correlation of a complex signal can be expressed as\begin{equation}\begin{split}r_{xx}(n) &= \mathbb E\bigg\{ x(k)x^*(k-n)\bigg\}\\r_{xx}(k-n) &= \mathbb E\bigg\{ x(k)x^*(k-n)\bigg\}\label{proof:corr}\end{split}\end{equation}Therefore, the Equation \ref{proof:periodogram} can be expressed as\begin{equation}P(\omega)=\lim\limits_{N \to \infty} \frac{1}{N} \sum_{n=0}^{N-1} \sum_{m=0}^{N-1}	r_{xx}(n-m)e^{-j(n-m)\omega}=\lim\limits_{N \to \infty} \frac{1}{N} \sum_{n=0}^{N-1} \sum_{m=0}^{N-1} g(n-m)\label{proof:rxx}\end{equation}Then, the double summation of Equation \ref{proof:rxx} could be converted into single one based on $\sum_{n=-N}^N \sum_{m=-N}^N g(n-m)=\sum_{k =-2N}^{2N}(2N+1-|k|)g(k)$. Thus, Equation \ref{proof:rxx} is \begin{align}P(\omega)&=\lim\limits_{N \to \infty} \frac{1}{N} \sum_{n=0}^{N-1} \sum_{m=0}^{N-1} g(n-m)\notag\\&=\lim\limits_{N \to \infty} \frac{1}{N} \sum_{k=-(N-1)}^{N-1}(N-|k|) g(k)\notag\\&=\sum_{k=-\infty}^{\infty} r_{xx}(k) e^{-jk\omega}  - \lim_{N\to\infty} \frac{1}{N} \sum_{k=-(N-1)}^{N-1} |k| r_{xx}(k) e^{-jk\omega}\label{proof:assump}\\&\approx \sum_{k=-\infty}^{\infty} r_{xx}(k) e^{-jk\omega} \  (under \ fast \ decays)\label{proof: final}\end{align}With the assumption of rapidly decays, the latter part of Equation \ref{proof:assump} tends to zero. Hence, the Equation \ref{proof:periodogram:starter} of PSD could be deduced to Equation \ref{proof: final}.